Engine: rename pike_vm_seen_state to pike_vm_state and PVSS to PVS

Engine/PikeSeenEquiv.v
@@ -475,7 +475,7 @@ Definition head_pc (threadactive:list thread) : label :=
   | (pc,_,_)::_ => pc
   end.
 
-Inductive pike_inv (code:code): pike_tree_seen_state -> pike_vm_seen_state -> Prop :=
+Inductive pike_inv (code:code): pike_tree_seen_state -> pike_vm_state -> Prop :=
 | pikeinv:
   forall inp treeactive treeblocked threadactive threadblocked best treeseen threadseen
     (ACTIVE: list_tree_thread code inp treeactive threadactive)
@@ -487,10 +487,10 @@ Inductive pike_inv (code:code): pike_tree_seen_state -> pike_vm_seen_state -> Pr
     (ENDTREE: advance_input inp forward = None -> treeblocked = [])
     (* any pc in threadseen must correspond to a tree in treeseen *)
     (SEEN: seen_inclusion code inp treeseen threadseen (hd_error treeactive) (head_pc threadactive)),
-    pike_inv code (PTSS inp treeactive best treeblocked treeseen) (PVSS inp threadactive best threadblocked threadseen)
+    pike_inv code (PTSS inp treeactive best treeblocked treeseen) (PVS inp threadactive best threadblocked threadseen)
 | pikeinv_final:
   forall best,
-    pike_inv code (PTSS_final best) (PVSS_final best).
+    pike_inv code (PTSS_final best) (PVS_final best).
 
 
 
@@ -816,7 +816,7 @@ Lemma initial_pike_inv:
     (TREE: bool_tree rer [Areg r] inp CanExit tree)
     (COMPILE: compilation r = code)
     (SUBSET: pike_regex r),
-    pike_inv code (pike_tree_seen_initial_state tree inp) (pike_vm_seen_initial_state inp).
+    pike_inv code (pike_tree_seen_initial_state tree inp) (pike_vm_initial_state inp).
 Proof.
   intros r inp tree code TREE COMPILE SUBSET.
   unfold compilation in COMPILE. destruct (compile r 0) as [c fresh] eqn:COMP.
@@ -838,10 +838,10 @@ Qed.
 (** * Invariant Preservation  *)
 
 (* identifying states of the VM that are going to take a skip step *)
-Definition skip_state (pvs:pike_vm_seen_state) : bool :=
+Definition skip_state (pvs:pike_vm_state) : bool :=
   match pvs with
-  | PVSS_final _ => false
-  | PVSS inp active best blocked seen =>
+  | PVS_final _ => false
+  | PVS inp active best blocked seen =>
       match active with
       | [] => false
       | (pc,gm,b)::active => inseenpc seen pc b
@@ -853,7 +853,7 @@ Theorem invariant_preservation:
   forall code pts1 pvs1 pvs2
     (STWF: stutter_wf code)
     (INV: pike_inv code pts1 pvs1)
-    (VMSTEP: pike_vm_seen_step rer code pvs1 pvs2),
+    (VMSTEP: pike_vm_step rer code pvs1 pvs2),
     (* either we make a step on both sides, preserving invariant *)
     (
       exists pts2,
@@ -870,7 +870,7 @@ Proof.
   inversion INV; subst.
   (* Final states make no step *)
   2: { inversion VMSTEP. }
-  destruct (skip_state (PVSS inp threadactive best threadblocked threadseen)) eqn:SKIP.
+  destruct (skip_state (PVS inp threadactive best threadblocked threadseen)) eqn:SKIP.
   (* skip states are performed in lockstep *)
   { left. destruct threadactive as [|[[pc gm] b] active]; simpl in SKIP.
     { inversion SKIP. }
@@ -894,7 +894,7 @@ Proof.
     inversion ACTIVE; subst.
     destruct treeblocked as [|[tblocked gmblocked] treeblocked].
     (* final step *)
-    - assert (pvs2 = (PVSS_final best)).
+    - assert (pvs2 = (PVS_final best)).
       { eapply pikevm_deterministic; eauto.
         destruct (advance_input inp) eqn:ADV; try solve[constructor; auto].
         specialize (BLOCKED i (eq_refl (Some i))). inversion BLOCKED; subst. constructor. }
@@ -903,7 +903,7 @@ Proof.
     - destruct (advance_input inp) eqn:ADV.
       2: { specialize (ENDTREE (eq_refl None)). inversion ENDTREE. }
       specialize (BLOCKED i (eq_refl (Some i))). inversion BLOCKED; subst.
-      assert (pvs2 = PVSS i ((pc,gmblocked,b)::threadlist) best [] initial_seenpcs).
+      assert (pvs2 = PVS i ((pc,gmblocked,b)::threadlist) best [] initial_seenpcs).
       { eapply pikevm_deterministic; eauto. constructor. auto. }
       subst. left. exists (PTSS i ((tblocked,gmblocked)::treeblocked) best [] initial_seentrees).
       apply advance_next in ADV. subst.
@@ -919,7 +919,7 @@ Proof.
     (* stuttering step *)
     right. apply stutter_step in TT as H; auto.
     destruct H as [nextpc [nextb [EPSSTEP TT2]]]; subst.
-    assert (pvs2 = (PVSS inp ([(nextpc, gm, nextb)] ++ threadactive) best threadblocked (add_thread threadseen (pc,gm,b)))).
+    assert (pvs2 = (PVS inp ([(nextpc, gm, nextb)] ++ threadactive) best threadblocked (add_thread threadseen (pc,gm,b)))).
     { eapply pikevm_deterministic; eauto. eapply pvss_active; eauto. }
     subst; simpl; auto. eapply pikeinv; simpl; eauto.
     - constructor; eauto.
@@ -929,7 +929,7 @@ Proof.
   destruct (tree_bfs_step t gm (idx inp)) eqn:TREESTEP.
   (* active *)
   - left. eapply generate_active in TREESTEP as H; eauto. destruct H as [newthreads [EPS LTT2]].
-    assert (pvs2 = PVSS inp (newthreads ++ threadactive) best threadblocked (add_thread threadseen (pc,gm,b))).
+    assert (pvs2 = PVS inp (newthreads ++ threadactive) best threadblocked (add_thread threadseen (pc,gm,b))).
     { eapply pikevm_deterministic; eauto. constructor; auto. }
     subst. exists (PTSS inp (l ++ treeactive) best treeblocked (add_seentrees treeseen t)). split.
     + eapply ptss_active; eauto.
@@ -937,14 +937,14 @@ Proof.
       apply ltt_app; eauto.
   (* match *)
   - left. eapply generate_match in TREESTEP as THREADSTEP; eauto.
-    assert (pvs2 = PVSS inp [] (Some (inp,gm_of (pc,gm,b))) threadblocked (add_thread threadseen (pc,gm,b))).
+    assert (pvs2 = PVS inp [] (Some (inp,gm_of (pc,gm,b))) threadblocked (add_thread threadseen (pc,gm,b))).
     { eapply pikevm_deterministic; eauto. constructor; auto. }
     subst. exists (PTSS inp [] (Some (inp,gm)) treeblocked (add_seentrees treeseen t)). split.
     + constructor; auto.
     + eapply pikeinv; try (eapply add_inclusion; eauto); try constructor; eauto.
   (* blocked *)
   - left. specialize (generate_blocked _ _ _ _ _ _ _ TREESTEP STUTTERS TT) as [EPS2 [TT2 [nexti ADVANCE]]].
-    assert (pvs2 = PVSS inp threadactive best (threadblocked ++ [(pc+1,gm,CanExit)]) (add_thread threadseen (pc,gm,b))).
+    assert (pvs2 = PVS inp threadactive best (threadblocked ++ [(pc+1,gm,CanExit)]) (add_thread threadseen (pc,gm,b))).
     { eapply pikevm_deterministic; eauto. constructor; auto. }
     subst. exists (PTSS inp treeactive best (treeblocked ++ [(t0,gm)]) (add_seentrees treeseen t)). split.
     + eapply ptss_blocked; eauto.
